Finished semantics plus added start of derivation

coq/tryingsometing.v
@@ -1,4 +1,6 @@
 Require Import ZArith List.
+Open Scope Z_scope.
+
 
 Variable string : Type.
 Variable lifetime : Type.
@@ -27,10 +29,18 @@ ae_num : forall r n, aeval r (anum n) (val n) (*n evaluates to n*)
 | ae_var1 : forall r x v, aeval ((x,v)::r) (avar x) v
 | ae_var2 : forall r x y v v1 , x <> y -> aeval r (avar x) v1 ->
 aeval ((y,v)::r) (avar x) v1
-(*| (*e1 + e2 evaluates to n1 + n2 if e1->n1 and e2->n2*) 
-ae_plus : forall r e1 e2 v1 v2,
-aeval r e1 (val v1) -> aeval r e2 (val v2) ->
-aeval r (aplus e1 e2) (v1 + v2)*).
+| (*e1 + e2 evaluates to n1 + n2 if e1->n1 and e2->n2*) 
+ae_plus : forall r e1 e2 v1 v2 w1 w2, 
+v1 = (val w1) -> v2 = (val w2) ->
+aeval r e1 v1 -> aeval r e2 v2 ->
+aeval r (aplus e1 e2) (val (w1 + w2))
+| (*either e1 or e2 evaluates to nothing*) 
+ae_plus_fail : forall r e1 e2 v1 v2, 
+v1 = nondec \/ v2 = nondec \/ v1 = dec \/ v2 = dec ->
+aeval r (aplus e1 e2) nondec
+(*| (*Not encountered yet*)
+ae_doesntmatter : forall e, aeval nil e nondec*)
+.
 
 
 (*When we want to update the state, we call this function*)
@@ -39,12 +49,79 @@ Inductive update : state -> string -> zext-> state -> Prop :=
 | s_up2 : forall r r1 x y v v1, update r x v1 r1 ->
 x <> y -> update ((y,v)::r) x v1 ((y,v)::r1).
 
+Definition usedvars := list string.
+
+Inductive findvars : usedvars -> aexpr -> usedvars -> Prop :=
+| try1: forall l x, findvars l (avar x) (x::l) (*variables*)
+| try2: forall l x y l1 l2, (findvars l x l1) -> (findvars l1 y l2) -> 
+findvars l (aplus x y) l2(*addition*)
+| try3: forall l i, findvars l (anum i) l(*integers*)
+.
+
+
+Inductive updateforev : state -> aexpr -> state -> Prop :=
+| try11: forall l x l1, update l x nondec l1 -> updateforev l (avar x) l1 (*variables*)
+| try21: forall l x y l1 l2, (updateforev l x l1) -> (updateforev l1 y l2) -> 
+updateforev l (aplus x y) l2(*addition*)
+| try31: forall l i, updateforev l (anum i) l(*integers*)
+.
 
 (*The actual natural semantics rules*)
 Inductive exec : state->instr->state->Prop :=
-| SN1 : forall r, exec r skip r
-| SN2 : forall r r1 x e v,
-aeval r e v -> update r x v r1 -> exec r (assign x e) r1
+| SN1 : forall r, exec r skip r (*skip rule*)
+| SN2 : forall r r1 x e v r2,
+aeval r e v -> update r x v r1 -> updateforev r1 e r2
+-> aeval r (avar x) dec (*A[x]s = dec*)
+-> not (aeval r e nondec)
+-> exec r (assign x e) r2
+(*assignment*)
+| SN4 : forall r x r1 r2 r3 y i a, (*s = r*)
+update r x dec r1 (*s[x |-> dec] = r1*)
+-> exec r1 i r2 (*<S, r1> -> r2 = s'*)
+-> aeval r (avar x) y (*r(x) = y = s(x)*)
+-> update r2 x y r3 (*r3 = s'[x |-> s(x)]*)
+-> exec r (let_in a x i) r3(*let-statement*)
 | SN3 : forall r r1 r2 i1 i2,
-exec r i1 r1 -> exec r1 i2 r2 ->
-exec r (sequence i1 i2) r2.
+exec r i1 r1 -> exec r1 i2 r2 
+-> exec r (sequence i1 i2) r2 (*composition*). 
+
+
+(*assign z (anum 5)*)
+Lemma Thalf:
+ forall z, exec ((z, dec)::nil) (assign z (anum 5)) ((z, val 5)::nil)
+.
+Proof.
+intros z.
+apply SN2 with (r1 := ((z,val 5)::nil)) (v := (val 5)).
+apply ae_num.
+apply s_up1.
+apply try31.
+apply ae_var1.
+admit. (*I get stuck here!*)
+Qed.
+
+(* let_in a (avar "z") (assign (avar "z") 5)
+let z in
+z := 5;
+*)
+
+Lemma T1:
+ forall z a, exec ((z, nondec)::nil) (let_in a z (assign z (anum 5))) ((z, nondec)::nil)
+.
+Proof.
+intros z. 
+intros a.
+apply SN4 with (r1 := ((z, dec)::nil)) (r2 := ((z, (val 5))::nil)) (y := nondec).
+apply s_up1.
+apply SN2 with (r1 := ((z, (val 5))::nil)) (v := (val 5)).
+apply ae_num.
+apply s_up1.
+apply try31.
+apply ae_var1.
+unfold not.
+admit.
+apply ae_var1.
+apply s_up1.
+Qed.
+
+
